LeanGrow/F/Prototypes/MarkFour/Frontend.lean
@@ -4,7 +4,7 @@ import Lean
 import LeanGrow.F.Utils.Expr.GetHyps
 import LeanGrow.F.Data.BuildDAG.ofTypeExpr
 import LeanGrow.F.Data.BuildDAG.SinksFirst
-import LeanGrow.F.Data.Unification.EmbedRawWInferWUnis
+--import LeanGrow.F.Data.Unification.EmbedRawWInferWUnis
 import LeanGrow.F.Prototypes.MarkFour.Search
 
 open Lean Elab Meta Command Tactic
@@ -17,7 +17,13 @@ def init_FixCtx (env : Environment) (init_gnodeTypes : Array CExpr) : FixCtx :=
   let T := env.constants.map₁.fold
     (fun sofar name info =>
       if (Name.isPrefixOf `Init modules[env.const2ModIdx[name].get! (α := Nat)]!) || (Name.isPrefixOf `LeanGrow.F.Prototypes.MarkOne.TestTypes modules[env.const2ModIdx[name].get! (α := Nat)]!)
-      then sofar.insert name.toString (ConstantInfo.toCstInfo env name info)
+      then
+      -- dbg
+        if (Name.isPrefixOf `LeanGrow.F.Prototypes.MarkOne.TestTypes modules[env.const2ModIdx[name].get! (α := Nat)]!)
+        then
+          dbg_trace s!"Addding {name} with type {repr info.type.toCExpr}"
+          sofar.insert name.toString (ConstantInfo.toCstInfo env name info)
+        else sofar.insert name.toString (ConstantInfo.toCstInfo env name info)
       else sofar
       )
     CTrie.empty
@@ -47,7 +53,7 @@ def Name_to_thmData (env : Environment) (n : Name) : Option miniPermiseDict :=
       let (Hs,G) := ThmType_ToDAG hs hs.length g
       let HS := SinksFirst Hs
       let (embD, orda) := mkEmbD (Array.mkArray HS.length default) #[] HS
-      .some ⟨n,embD,orda,G.1⟩
+      .some ⟨.none,n,embD,orda,G.1⟩
 
 
 def Names_to_thmData (env : Environment) (L : List Name) : List miniPermiseDict :=
@@ -75,11 +81,103 @@ def LCtx_to_ltx_and_goal (ctx : LocalContext) : List (Nat × CExpr) × CExpr :=
       (Hs.map (fun (a,b,_) => (a,Gnodify b)), Gnodify G.1)
 
 
+-- New: ∀ in hyps interpreted as premises
+
+def CExpr.getHypsGoal (ty : CExpr) : (List (CExpr × Bool)) × CExpr :=
+  let rec go (cache : List (CExpr × Bool)) : CExpr → (List (CExpr × Bool)) × CExpr
+    | .forallE _ h b i =>
+          match i with
+          | .instImplicit => go ((h , true) :: cache) b
+          | _ => go ((h , false) :: cache) b
+    | e => (cache, e)
+  go [] ty
+
+
+partial def cThmType_ToDAG (hyps : List (CExpr × Bool)) (l_len : Nat) (goal : CExpr) : List (Nat × CExpr × Bool × List Nat) × (CExpr × List Nat) :=
+  let inc_helper : Option Nat → Option Nat
+    | .none => .some 0
+    | .some x => .some (x+1)
+  let rec abstractBvars_collectParents (E : CExpr) (offset : Nat → Nat) : CExpr × List Nat :=
+    let rec go1 (offset : Nat → Nat) (cache_pars : (List Nat)) (dinfo : List (Option Nat)) : List CExpr → (List CExpr) × List Nat
+      | [] =>
+          ([], cache_pars)
+      | e :: more =>
+          match e with
+          | .app (.app (.const `optParam _) e) _ => go1 offset cache_pars dinfo (e :: more)  -- got wierd problems in source file gen otherwise
+          | .app (.app (.const `outParam _) e) _ => go1 offset cache_pars dinfo (e :: more)
+          | .bvar i =>
+                let (d?,ndi) := List.headD_tail dinfo .none
+                match d? with
+                | .none =>
+                    let (re,rp) := go1 offset (List.orderedInsertOrLeave (· ≤ · ) (offset (i+1)) cache_pars) ndi more
+                    (((CExpr.lnode (offset (i+1))) (.ofBvar i) .none) :: re, rp)
+                | .some d =>
+                    if i ≤ d
+                    then
+                      let (re,rp) := go1 offset cache_pars ndi more
+                      ((.bvar i) :: re, rp)
+                    else
+                      let (re,rp) := go1 offset (List.orderedInsertOrLeave (· ≤ · ) (offset (i - d)) cache_pars) ndi more
+                      (((CExpr.lnode (offset (i - d))) (.ofBvar i) .none) :: re, rp)
+          | .app l r => let d? := List.headD dinfo .none
+                        let (re,rp) := go1 offset cache_pars (d? :: dinfo) (l :: r :: more)
+                        let (L,re2) := List.headD_tail re .failed
+                        let (R,re3) := List.headD_tail re2 .failed
+                        (.app L R :: re3, rp)
+          | .lam n l r B => let (d?,ndi) := List.headD_tail dinfo .none
+                            let (re,rp) := go1 offset cache_pars (d? :: (inc_helper d?) :: ndi) (l :: r :: more)
+                            let (L,re2) := List.headD_tail re .failed
+                            let (R,re3) := List.headD_tail re2 .failed
+                            (.lam n L R B :: re3, rp)
+          | .forallE n l r B => let (d?,ndi) := List.headD_tail dinfo .none
+                                let (re,rp) := go1 offset cache_pars (d? :: (inc_helper d?) :: ndi) (l :: r :: more)
+                                let (L,re2) := List.headD_tail re .failed
+                                let (R,re3) := List.headD_tail re2 .failed
+                                (.forallE n L R B :: re3, rp)
+          | .proj n i e => let (re,rp) := go1 offset cache_pars dinfo (e :: more)
+                           let (E,r2) :=  List.headD_tail re .failed
+                           (.proj n i E :: r2, rp)
+          -- we don't expect `let` or mvar or fvars in thm types ...
+          | x =>
+              let ndi := List.tailD dinfo []
+              let (cs, ps) := go1 offset cache_pars ndi (more)
+              (x :: cs, ps)
+    let (ce, ps) := go1 offset [] [.none] [E]
+    (List.headD ce .failed, ps)
+  let rec go2 (l : List (CExpr × Bool)) (count : Nat) (cache : List (Nat × CExpr × Bool × List Nat)) : List (Nat × CExpr × Bool × List Nat) × (CExpr × List Nat) :=
+    match l with
+    | [] =>
+        let (res, deps) := abstractBvars_collectParents goal (fun o => l_len - o)
+        (cache, (res, deps))
+    | h :: rest =>
+          let (res, deps) := abstractBvars_collectParents h.1 (fun o => count - o)
+          go2 rest (count - 1) (⟨count, res, h.2, deps⟩ :: cache)
+  go2 hyps (l_len - 1) []
+
+
+def AllHyp_to_thmData (gid : Nat) (type : CExpr) : Option miniPermiseDict :=
+  let rec mkEmbD (thmD : Array EmbedData) (thmO : Array Nat) : List (ℕ × CExpr × Bool × List ℕ) → (Array EmbedData × Array Nat)
+    | [] => (thmD, thmO)
+    | nx :: more =>
+        if nx.2.2.1
+        then mkEmbD (thmD.set! nx.1 (.inst nx.2.1 #[] #[])) (thmO.push nx.1) more
+        else mkEmbD (thmD.set! nx.1 (.nonInst nx.2.1 #[] #[])) (thmO.push nx.1) more
+        -- push is to the right, so order is preserved
+        -- parent and child datat turned out useless
+  match type with
+  | .forallE _ _ _ _ =>
+      let (hs,g) := type.getHypsGoal
+      let (Hs,G) := cThmType_ToDAG hs hs.length g
+      let HS := SinksFirst Hs
+      let (embD, orda) := mkEmbD (Array.mkArray HS.length default) #[] HS
+      .some ⟨.some gid, `dummy ,embD,orda,G.1⟩
+  | _ => .none
+
 
 
 elab "grow" : tactic => do
   let ref ← getRef
-  let dEnv ← simpleImportModules #[`LeanGrow.F.Prototypes.MarkOne.TestTypes]
+  let dEnv ← simpleImportModules #[`LeanGrow.F.Prototypes.MarkFour.TestTypes]
   Elab.Tactic.withMainContext do
     let Ltx ←  getLCtx
 
@@ -88,11 +186,12 @@ elab "grow" : tactic => do
         (fun sofar (idx,exp) => PageingSet sofar (fun x => (x / 42, x % 42)) 42 (.failed) idx exp)
         []
     let fctx := init_FixCtx dEnv (ltx.map Prod.snd).toArray
-    --
-    let premises :=(Names_to_thmData dEnv [`myAdd_zero, `Eq.trans].reverse)
-    let st : SearchState := ⟨⟨0,1,0,[(0,goal)], .ofGoal 0 goal [] [] [] ⟩, ltx, forw2, (fun x => (x / 42, x % 42)), ltx.length, fctx, [], [], [],[],[]⟩
+    dbg_trace s!"Test {repr (CExpr.inferType fctx (.const `List.sum []))}"
+    let outer_premises := (Names_to_thmData dEnv [`Nat.dvd_trans, `PremOne].reverse)
+    let inner_premises := (ltx.map (fun (n,ce) => AllHyp_to_thmData n ce)).reduceOption
+    let st : SearchState := ⟨⟨0,1,0,[(0,goal)], .ofGoal 0 goal [] [] [] ⟩, .leaf [0] ltx, forw2, (fun x => (x / 42, x % 42)), ltx.length, fctx, [], [], [],[],[]⟩
     --logInfoAt ref s!"{repr premises}"
-    let res := search 20 premises st
+    let res := search 20 (inner_premises ++ outer_premises) st
     match res with
     | .none => logInfoAt ref "nope"
     | .some res! => logInfoAt ref s!"Recovered : {repr res!}"
